\chapter{Detailed Calculation}
\subsection{Lemma \ref{lemma:rhok}}
The characteristic equation is:
\begin{equation}
A-\lambda I=\begin{pmatrix}
\frac{1}{2 a}-\lambda & \frac{2}{a^2} \\
1             & -\lambda 
\end{pmatrix}\;
=\lambda^2-\frac{1}{2 a}\lambda-\frac{2}{a^2}=0
\end{equation}
which solved for $\lambda$ gets the claimed eigenvalues.

We know that $\vect{v}_1 = A \vect{v}_1  $, which is:
\begin{equation}
\begin{pmatrix}
x \\ 
y 
\end{pmatrix}\;
=
\begin{pmatrix}
\frac{1}{2 a} & \frac{2}{a^2} \\
1             & 0 
\end{pmatrix}\;
\begin{pmatrix}
x \\ 
y 
\end{pmatrix}\;
\end{equation}
By calculation:
\begin{flalign}
\label{eqn:xany}x &= \frac{1}{2 a}x+\frac{2}{a^2}y\\
\label{eqn:xey} y &= x
\end{flalign}
By \eqref{eqn:xany}, we could find $x$ could be any value. 
We already know that $\vect{v}_1$ is a unit vector.

Because $A \vect{v}_2 = \lambda_2 \vect{v}_2$. Thus we could find:
\begin{equation}
\lambda_2
\begin{pmatrix}
x \\ 
y 
\end{pmatrix}\;
= 
\begin{pmatrix}
\frac{1}{2 a} & \frac{2}{a^2} \\
1             & 0 
\end{pmatrix}\;
\begin{pmatrix}
x \\ 
y 
\end{pmatrix}\;
\end{equation}
By calculation, 
\begin{flalign}
\label{eqn:xany2}\lambda_2 x &= \frac{1}{2 a}x+\frac{2}{a^2}y\\
\label{eqn:x2ey}\lambda_2 y &=  x
\end{flalign}
Therefore we could get:
$$\vect{v}_2 = 
\frac{1}{\sqrt{\lambda_2^2+1}}
\begin{pmatrix}
\lambda_2\\
1
\end{pmatrix}$$

The system of equation becomes:
$$\frac{\sqrt{2}}{2}\rho+\frac{\lambda_2}{\sqrt{1+\lambda_2^2}}\alpha = \rho_2 $$
$$\frac{\sqrt{2}}{2}\rho\lambda_2+\frac{\lambda_2}{\sqrt{1+\lambda_2^2}}\alpha = \rho_1\lambda_2$$
and subtracting the second equation from the first:
$$\rho=\frac{\rho_1\lambda_2-\rho_2}{\frac{\sqrt{2}}{2}(\lambda_2-1)}=\frac{40+8\sqrt{33}}{\sqrt{66}+33\sqrt{2}}\approx1.5687$$

\subsection{Lower Bound Comparison}
Since
$$\rho = \frac{20 \sqrt{2} + 4 \sqrt{66}}{\sqrt{66} + 33 \sqrt{2}}\;,$$
$$a = (1 + \sqrt{33}) / 4\;,$$
and the previous lower bound is $(2-p)^k$ where $p = (3-\sqrt{5})/2$. 
Then,
$$\lim_{k \rightarrow \infty} \frac{\rho\alpha^k}{(2 - p)^k} = \infty\;,$$
which implies that the new lower bound is strictly tighter than the previous one.

